prove that expand' is idempotent

hygiene.lean
@@ -14,14 +14,130 @@ using_well_founded { dec_tac := tactic.admit }
 def α_equiv (rsm : resolve_map) (s₁ s₂ : syntax) :=
 ∃ σ, α_conv rsm σ s₁ = s₂
 
-protected def except.assert {ε} : except ε Prop → Prop
+protected def except.passert {ε} : except ε Prop → Prop
 | (except.ok p)    := p
-| (except.error _) := false
+| (except.error _) := true
+
+namespace parse_m
+variables {r σ α : Type} (cfg : r) (st : σ)
+
+protected def passert := except.passert ∘ parse_m.run' cfg st
+
+protected def passert' (x : parse_m r σ α) (p : σ → α → Prop) :=
+match parse_m.run cfg st x : _ → Prop with
+| except.ok ⟨a, st'⟩ := p st' a
+| except.error _    := true
+end
+
+variables {cfg st}
+
+protected lemma passert_passert' (x : parse_m r σ Prop) :
+  parse_m.passert cfg st x = parse_m.passert' cfg st x (λ st a, a) := sorry
+
+variable (x : parse_m r σ α)
+
+@[simp] lemma passert'_pure (a : α) (p) : parse_m.passert' cfg st (pure a) p = p st a := sorry
+
+@[simp] lemma passert'_bind {β}
+  (f : α → parse_m r σ β) (p : σ → β → Prop) :
+  parse_m.passert' cfg st (x >>= f) p =
+  parse_m.passert' cfg st x (λ st' a, parse_m.passert' cfg st' (f a) p) := sorry
+
+@[simp] lemma passert'_fmap {β}
+  (f : α → β) (p : σ → β → Prop) :
+  parse_m.passert' cfg st (f <$> x) p =
+  parse_m.passert' cfg st x (λ st' a, p st' (f a)) := sorry
+
+@[simp] lemma passert'_with_state {σ'} (f : σ → σ') (p) (x : parse_m r σ' α) :
+  parse_m.passert' cfg st (with_state f x) p = parse_m.passert' cfg (f st) x (λ _, p st) := sorry
+
+@[simp] lemma passert'_read (p) :
+  parse_m.passert' cfg st (read) p = p st st := sorry
+
+@[simp] lemma passert'_write (p st') :
+  parse_m.passert' cfg st (write st') p = p st' punit.star := sorry
+
+@[simp] lemma passert'_reader_t_read (p) :
+  parse_m.passert' cfg st (reader_t.read) p = p st cfg := sorry
+
+lemma passert'_mp {p : parse_m r σ α} {s₀ : σ} {post₁ post₂ : σ → α → Prop} :
+     parse_m.passert' cfg s₀ p post₁ → (∀ s a, post₁ s a → post₂ s a) → parse_m.passert' cfg s₀ p post₂ :=
+sorry /-begin
+  simp [passert],
+  generalize h₁ : p s₀ = o,
+  cases o with r,
+  { simp [passert] },
+  { cases r with a s,
+    simp [passert], intros h₁ h₂, exact h₂ _ _ h₁ }
+end-/
+
+lemma passert'_mp_no_state {p : parse_m r σ α} {s₀ s₀' : σ} {post₁ post₂ : α → Prop} :
+     parse_m.passert' cfg s₀ p (λ s, post₁) → (∀ a, post₁ a → post₂ a) → parse_m.passert' cfg s₀' p (λ s, post₂) :=
+sorry
+end parse_m
 
 theorem hygienic (s₁ s₂ : syntax) (st : parse_state) :
-except.assert $ parse_m.run' st () $
-(do s₁' ← expand' s₁,
-    s₂' ← expand' s₂,
-    (_, rst) ← resolve' s₁',
-    pure $ α_equiv rst.resolve_map s₁ s₂ → α_equiv rst.resolve_map s₁' s₂')
-:= sorry
+parse_m.passert st () $
+do s₁' ← expand' s₁,
+   s₂' ← expand' s₂,
+   (_, rst) ← resolve' s₁',
+   pure $ α_equiv rst.resolve_map s₁ s₂ → α_equiv rst.resolve_map s₁' s₂' := sorry
+
+lemma expand_idem (s : syntax) (cfg : parse_state) :
+parse_m.passert cfg () $
+do s' ← expand' s,
+   s'' ← expand' s',
+   pure $ s'' = s' :=
+begin
+  -- generalize states (irrelevant) and step counts
+  suffices : ∀ st st₂ steps steps₂, steps ≤ steps₂ → parse_m.passert' cfg st (expand steps s)
+    (λ (_x : expand_state) (a : syntax),
+       parse_m.passert' cfg st₂ (expand steps₂ a) (λ (_x : expand_state) (a_1 : syntax), a_1 = a)),
+  { simp [parse_m.passert_passert', expand'], apply this, apply le_refl },
+  intros st st₂ steps steps₂,
+  induction steps with steps generalizing s st st₂ steps₂,
+  -- `expand s` out of steps: trivial
+  { intros; simp [expand] },
+  { intro hsteps₂,
+    -- `expand s'` can do at least one step as well
+    cases steps₂ with steps₂, { exfalso, apply nat.not_succ_le_zero _ hsteps₂ },
+    -- recursive case 1: holds when expanding all children (when s is not a macro)
+    have expand_mmap : ∀ (val : syntax_node syntax),
+      parse_m.passert' cfg st (mmap (expand steps) (val.args))
+        (λ (st' : expand_state) (a_1 : list syntax),
+          parse_m.passert' cfg st₂ (mmap (expand steps₂) a_1)
+            (λ (st' : expand_state) (a : list syntax),
+                syntax.node {id := val.id, sp := val.sp, m := val.m, args := a} =
+                  syntax.node {id := val.id, sp := val.sp, m := val.m, args := a_1})),
+    begin
+        intro,
+        induction val.args generalizing st st₂; simp [mmap],
+        case list.cons {
+          apply parse_m.passert'_mp (ih_1 _ st st₂ _ (nat.le_of_succ_le_succ hsteps₂)), intros st' s' expand_s',
+          apply parse_m.passert'_mp (ih_1_1 st' st₂), intros st'' args' mmap_args',
+          apply parse_m.passert'_mp expand_s', intros st''' s''' _,
+          apply parse_m.passert'_mp_no_state mmap_args', intros args this,
+          -- TODO: use whnf_ginductive in injection
+          apply syntax.node.inj_arrow this, intro this, injection this,
+          simp *
+        }
+    end,
+    cases hs : s; simp [expand],
+    --TODO `case` for ginductives
+    --case syntax.node n {
+    { cases h : rbmap.find cfg.macros val.m with m,
+      case none { simp [expand, h], apply expand_mmap },
+      case some {
+        cases m, cases expand,
+        case none { simp [expand, h], apply expand_mmap },
+        case some {
+          -- recursive case 1: re-expand the expansion of s. `expand s` will do one more step than `expand s'`.
+          -- `mk_tag` is so simple that `simp` can automatically transform it to its spec
+          simp [expand, mk_tag],
+          apply parse_m.passert'_mp (ih_1 _ _ st₂ _ (nat.le_of_succ_le hsteps₂)), intros st' s' expand_s',
+          apply expand_s',
+        },
+      }
+    }
+  }
+end
